theories/Lang/StImpS.v
@@ -1,0 +1,180 @@
+From Coq Require Import
+  PeanoNat
+  Lia.
+
+From ExtLib Require Import
+  Structures.Maps
+  RelDec
+  Data.Map.FMapAList
+  Data.String.
+
+From TICL Require Import
+  ICTree.Core
+  ICTree.SBisim
+  ICTree.Equ
+  ICTree.Interp.State
+  ICTree.Events.State
+  ICTree.Events.Writer
+  Logic.Trans
+  Logic.Core
+  ICTree.Logic.AX
+  ICTree.Logic.AF
+  ICTree.Logic.EX
+  ICTree.Logic.EF
+  ICTree.Logic.Bind
+  ICTree.Logic.CanStep
+  ICTree.Logic.State
+  Lang.Maps.
+
+Generalizable All Variables.
+
+Import ICtree ICTreeNotations TiclNotations.
+Local Open Scope ticl_scope.
+Local Open Scope ictree_scope.
+Local Open Scope nat_scope.
+
+Generalizable All Variables.
+
+Module ME.
+  (*| Security labels |*)
+  Variant Sec: Set := H | L.
+  
+  (*| Preorder of [sec] labels |*)
+  Reserved Notation "a ≺ b" (at level 52, left associativity).
+  Variant sec_lt: relation Sec :=
+    | SecLt: L ≺ H
+  where "a ≺ b" := (sec_lt a b).
+  Local Hint Constructors sec_lt: core.
+  
+  Reserved Notation "a ⪯ b" (at level 52, left associativity).
+  Variant sec_lte: relation Sec :=
+    | SecRefl: forall a, a ⪯ a
+    | SecHL: L ≺ H -> L ⪯ H
+  where "a ⪯ b" := (sec_lte a b).
+  Local Hint Constructors sec_lte: core.
+  
+  Local Instance sec_lte_refl: Reflexive sec_lte := SecRefl.
+  Local Instance sec_lt_trans: Transitive sec_lt.
+  Proof.
+    red; intros [] [] [] *; auto; intros.
+    inv H0. inv H1.
+  Qed.
+  
+  Local Instance sec_lte_trans: Transitive sec_lte.
+  Proof. red; intros [] [] [] *; auto. Qed.
+  
+  Lemma sec_lte_dec(l r: Sec): { l ⪯ r } + { r ≺ l }.
+  Proof.
+    revert r; induction l; destruct r.
+    - left; reflexivity. 
+    - right; auto. 
+    - left; auto.
+    - left; reflexivity.
+  Qed.
+  
+  Lemma sec_lte_H(l: Sec): l ⪯ H.
+  Proof. destruct l; repeat econstructor. Qed.
+  
+  Lemma sec_lte_L(l: Sec): L ⪯ l.
+  Proof. destruct l; repeat econstructor. Qed.
+  
+  (*| Both values and addresses are nat |*)
+  Notation Addr := nat.
+  
+  Variant secE: Type :=
+    | Read (l: Sec) (addr: Addr)
+    | Write (l: Sec) (addr: Addr) (val: nat).
+  
+
+  (* Secure tagged heaps *)
+  Context `{MF: Map Addr (Sec * nat) St} `{OF: MapOk Addr (Sec * nat) St eq}.
+  
+  Global Instance encode_secE: Encode secE :=
+    fun e => match e with
+          | Read l addr => option nat
+          | Write l addr v => unit
+          end.
+  
+  (* Ghost state, instrument every read with
+     [m: memory address it targets]
+     [ml: Security-level of the instruction]
+     [al: Security-level of the address cell previously written]
+   *)               
+  Record SecObs := { ml: Sec; al: Sec }.
+
+  (* Insecure interpreter, does not check labels *)
+  Definition h_secE: secE ~> stateT St (ictreeW SecObs) :=
+    fun e => mkStateT
+            (fun (st: St) =>                                     
+               match e return ictreeW SecObs (encode e * St) with
+               | Read l addr =>
+                   match lookup addr st with
+                   (* [addr] exists and set to [(v, l_a)] *)
+                   | Some (l_a, v) =>
+                       (* Instrumentation *)
+                       log {| ml:=l_a; al := l |} ;;
+                       Ret (Some v, st)
+                   (* [addr] does not exist, return [None] *)
+                   | None => Ret (None, st)
+                   end
+               | Write l addr v =>
+                   (* Set [addr] to [(l, v)] *)
+                   Ret (tt, add addr (l, v) st)
+               end).
+
+  (* Client program *)
+  Inductive CProg : Type -> Type :=
+  | CRead (l: Sec) (addr: Addr): CProg (option nat)
+  | CWrite (l: Sec) (addr: Addr) (v: nat): CProg unit
+  | CIf {A B X} (c: {A} + {B}) (t: CProg X) (e: CProg X): CProg X
+  | CRet {A}(a: A): CProg A
+  | CBind {A B}(l: CProg A) (k: A -> CProg B): CProg B.
+
+  Fixpoint denote_cprog {A}(s: CProg A): ictree secE A :=
+    match s with
+    | CRead l addr => ICtree.trigger (Read l addr)
+    | CWrite l addr v => ICtree.trigger (Write l addr v)
+    | CIf c t e =>
+        if c then
+          denote_cprog t
+        else
+          denote_cprog e
+    | CRet x => Ret x
+    | CBind l k =>
+        x <- denote_cprog l ;;        
+        denote_cprog (k x)
+    end.
+
+  (* Scheduler program *)
+  Inductive SProg: Type -> Type :=
+  | SLoop {X}(i: X) (b: X -> SProg X): SProg unit
+  | SBr {X} (l r: SProg X): SProg X
+  | SCall {X} (p: CProg X): SProg X
+  | SRet {A}(a: A): SProg A
+  | SBind {A B}(l: SProg A) (k: A -> SProg B): SProg B.
+
+  Fixpoint denote_sprog {A}(s: SProg A): ictree secE A :=
+    match s with
+    | @SLoop X i b =>
+        ICtree.iter
+          (fun (i: X) =>
+             x <- denote_sprog (b i) ;;
+             Ret (inl x)) i
+    | SBr l r =>
+        ICtree.br2 (denote_sprog l) (denote_sprog r)
+    | SCall p => denote_cprog p
+    | SRet x => Ret x
+    | SBind l k =>
+        x <- denote_sprog l ;;        
+        denote_sprog (k x)
+    end.
+
+  (* Instrumentation of client programs *)
+  Definition instr_cprog {X}(p: CProg X): St -> ictreeW SecObs (X * St) :=
+    interp_state h_secE (denote_cprog p).
+
+  (* Instrumentation of scheduler programs *)
+  Definition instr_sprog {X}(p: SProg X): St -> ictreeW SecObs (X * St) :=
+    interp_state h_secE (denote_sprog p).
+  
+End ME.
